src/dafny/beacon/statetransition/stateTransition.cap.dfy
@@ -1,0 +1,128 @@
+include "../../utils/Eth2Types.dfy"
+include "../../utils/MathHelpers.dfy"
+include "../../ssz/Constants.dfy"
+include "../BeaconChainTypes.dfy"
+include "../Helpers.dfy"
+include "../Helpers.s.dfy"
+include "../Helpers.cap.dfy"
+include "../validators/Validators.dfy"
+include "StateTransition.s.dfy"
+include "EpochProcessing.dfy"
+include "ProcessOperations.dfy"
+include "ProcessOperations.s.dfy"
+
+
+
+module  StateTransitionCapella {
+
+    //  Import some constants, types and beacon chain helpers.
+    import opened Eth2Types
+    import opened MathHelpers
+    import opened Constants
+    import opened BeaconChainTypes
+    import opened BeaconHelpers
+    import opened BeaconHelperSpec
+    import opened BeaconHelpersCapella
+    import opened Validators
+    import opened StateTransitionSpec
+    import opened EpochProcessing
+    import opened ProcessOperations
+    import opened ProcessOperationsSpec
+
+
+    method get_expected_withdrawals(s: BeaconState) returns (withdrawals: seq<Withdrawal>)
+            requires |s.validators| == |s.balances|
+            requires minimumActiveValidators(s)
+            requires s.next_withdrawal_validator_index as int < |s.validators|
+
+            {
+                var epoch := get_current_epoch(s);
+                // var withdrawal_index := s.next_withdrawal_index;
+                // var validator_index := s.next_withdrawal_validator_index;
+                withdrawals := [];
+                var bound := min(|s.validators|, MAX_VALIDATORS_PER_WITHDRAWAL_SWEEP as nat) as nat;
+                var i: int;
+
+                for i := 0 to bound - 1 {
+                    var validator := s.validators[s.next_withdrawal_validator_index];
+                    var balance := s.balances[s.next_withdrawal_validator_index];
+                    // var addressBytes := validator.withdrawal_credentials.bs[12..32];
+                    // var address: ExecutionAddress := addressBytes;
+                    var newNextWithdrawalValidatorIndex := s.next_withdrawal_validator_index as int;
+                    if is_fully_withdrawable_validator(validator, balance, epoch) {
+                        var withdrawal := Withdrawal(
+                            index := s.next_withdrawal_validator_index,
+                            validator_index := s.next_withdrawal_validator_index,
+                            address := validator.execution_address,
+                            amount := balance
+                        );
+                        withdrawals := withdrawals + [withdrawal];
+                        // s.next_withdrawal_validator_index := s.next_withdrawal_validator_index + 1;
+                        newNextWithdrawalValidatorIndex := s.next_withdrawal_validator_index as int + 1;
+                    } else if is_partially_withdrawable_validator(validator, balance, epoch) {
+                        var withdrawal := Withdrawal(
+                            index := s.next_withdrawal_validator_index,
+                            validator_index := s.next_withdrawal_validator_index,
+                            address := validator.execution_address,
+                            amount := balance - MAX_EFFECTIVE_BALANCE
+                        );
+                        withdrawals := withdrawals + [withdrawal];
+                        // s.next_withdrawal_validator_index := s.next_withdrawal_validator_index + 1;
+                        newNextWithdrawalValidatorIndex := s.next_withdrawal_validator_index as int + 1;
+                    }
+
+                    if |withdrawals| == MAX_WITHDRAWALS_PER_PAYLOAD as int {
+                        break;
+                    }
+
+                    // s.next_withdrawal_validator_index := (s.next_withdrawal_validator_index + 1) % |s.validators|;
+                    newNextWithdrawalValidatorIndex := (newNextWithdrawalValidatorIndex + 1) % |s.validators|;
+                }
+
+            }
+
+
+    
+        
+    // method process_withdrawals(state: BeaconState, payload: ExecutionPayload)
+    // {
+    //     var expected_withdrawals := get_expected_withdrawals(state);
+    //     assert |payload.withdrawals| == |expected_withdrawals|;
+
+    //     var newNextWithdrawalIndex := state.next_withdrawal_index;
+    //     var newNextValidatorIndex := state.next_withdrawal_validator_index;
+
+
+    //     for i := 0 to |expected_withdrawals| - 1 {
+    //         var expected_withdrawal := expected_withdrawals[i];
+    //         var withdrawal := payload.withdrawals[i];
+    //         assert withdrawal == expected_withdrawal; // Verify that elements match
+
+    //         // Call decrease_balance method with state, withdrawal.validator_index, and withdrawal.amount
+    //         BeaconState() := decrease_balance(state, expected_withdrawal.validator_index, expected_withdrawal.amount);
+    //     }
+
+    //     // Update the next withdrawal index if this block contained withdrawals
+    //     if |expected_withdrawals| != 0 {
+    //         var latest_withdrawal := expected_withdrawals[|expected_withdrawals| - 1];
+    //         newNextWithdrawalIndex := latest_withdrawal.index + 1;
+    //     }
+
+    //     // Update the next validator index to start the next withdrawal sweep
+    //     if |expected_withdrawals| == MAX_WITHDRAWALS_PER_PAYLOAD as int {
+    //         // Next sweep starts after the latest withdrawal's validator index
+    //         var next_validator_index := (expected_withdrawals[|expected_withdrawals| - 1].validator_index + 1) % |state.validators|;
+    //         newNextValidatorIndex := next_validator_index;
+    //     } else {
+    //         // Advance sweep by the max length of the sweep if there was not a full set of withdrawals
+    //         var next_index := (state.next_withdrawal_validator_index + MAX_VALIDATORS_PER_WITHDRAWALS_SWEEP) as int;
+    //         var next_validator_index := next_index % |state.validators|;
+    //         newNextValidatorIndex := next_validator_index; 
+    //     }
+    // }
+
+
+    // method process_
+
+}
+    
